New optimizations

ver2/optimizations/eq_zero.v
@@ -56,11 +56,12 @@ Require Import List.
 Import ListNotations.
 
 
-Module Opt_add_zero.
+Module Opt_eq_zero.
 
 
-(* ADD(X,0) or ADD(0,X) = X *)
-Definition optimize_add_0_sbinding : opt_smap_value_type := 
+(* EQ(X,0) = ISZERO(X)
+   EQ(0,X) = ISZERO(X) *)
+Definition optimize_eq_zero_sbinding : opt_smap_value_type := 
 fun (val: smap_value) =>
 fun (fcmp: sstack_val_cmp_t) =>
 fun (sb: sbindings) =>
@@ -68,132 +69,126 @@ fun (maxid: nat) =>
 fun (instk_height: nat) =>
 fun (ops: stack_op_instr_map) => 
 match val with
-| SymOp ADD [arg1; arg2] => 
+| SymOp EQ [arg1; arg2] => 
   if fcmp arg1 (Val WZero) maxid sb maxid sb instk_height ops then
-    (SymBasicVal arg2, true)
+    (SymOp ISZERO [arg2], true)
   else if fcmp arg2 (Val WZero) maxid sb maxid sb instk_height ops then
-    (SymBasicVal arg1, true)
+    (SymOp ISZERO [arg1], true)
   else
     (val, false)
 | _ => (val, false)
 end.
 
 
+Lemma eq_zero_iszero1: forall (x: EVMWord) ctx,
+evm_eq ctx [WZero; x] = evm_iszero ctx [x].
+Proof.
+intros. unfold evm_iszero. 
+rewrite -> eq_comm. reflexivity.
+Qed.
+
+Lemma eq_zero_iszero2: forall (x: EVMWord) ctx,
+evm_eq ctx [x; WZero] = evm_iszero ctx [x].
+Proof.
+intros. unfold evm_iszero. 
+rewrite -> eq_comm. reflexivity.
+Qed.
 
 
 
 
-Lemma optimize_add_0_sbinding_smapv_valid:
-opt_smapv_valid_snd optimize_add_0_sbinding.
+Lemma optimize_eq_zero_sbinding_smapv_valid:
+opt_smapv_valid_snd optimize_eq_zero_sbinding.
 Proof.
 unfold opt_smapv_valid_snd.
 intros instk_height n fcmp sb val val' flag.
-intros Hvalid_smapv_val Hvalid_sb Hoptm_add_0_sbinding.
-unfold optimize_add_0_sbinding in Hoptm_add_0_sbinding.
+intros Hvalid_smapv_val Hvalid_sb Hoptm_eq_zero_sbinding.
+unfold optimize_eq_zero_sbinding in Hoptm_eq_zero_sbinding.
 destruct (val) as [basicv|pushtagv|label args|offset smem|key sstrg|
   offset size smem] eqn: eq_val.
-+ injection Hoptm_add_0_sbinding as eq_val' eq_flag.
++ injection Hoptm_eq_zero_sbinding as eq_val' eq_flag.
   rewrite <- eq_val'.
   assumption.
-+ injection Hoptm_add_0_sbinding as eq_val' eq_flag.
++ injection Hoptm_eq_zero_sbinding as eq_val' eq_flag.
   rewrite <- eq_val'.
   assumption.
 + destruct label eqn: eq_label; try 
-      (injection Hoptm_add_0_sbinding as eq_val' eq_flag;
+      (injection Hoptm_eq_zero_sbinding as eq_val' eq_flag;
       rewrite <- eq_val'; assumption).
   (* ADD *)
   destruct args as [|arg1 r1] eqn: eq_args; try 
-    (injection Hoptm_add_0_sbinding as eq_val' eq_flag;
+    (injection Hoptm_eq_zero_sbinding as eq_val' eq_flag;
     rewrite <- eq_val'; assumption).
   destruct r1 as [|arg2 r2] eqn: eq_r1; try 
-    (injection Hoptm_add_0_sbinding as eq_val' eq_flag;
+    (injection Hoptm_eq_zero_sbinding as eq_val' eq_flag;
     rewrite <- eq_val'; assumption).
-  destruct r2 as [|arg3 r3] eqn: eq_r2; try 
-    (injection Hoptm_add_0_sbinding as eq_val' eq_flag;
+  destruct r2; try 
+    (injection Hoptm_eq_zero_sbinding as eq_val' eq_flag;
     rewrite <- eq_val'; assumption).
   destruct (fcmp arg1 (Val WZero) n sb n sb instk_height evm_stack_opm)
     eqn: eq_fcmp_arg1.
-  * injection Hoptm_add_0_sbinding as eq_val' eq_flag.
+  * injection Hoptm_eq_zero_sbinding as eq_val' eq_flag.
     rewrite <- eq_val'.
     simpl in Hvalid_smapv_val. unfold valid_stack_op_instr in Hvalid_smapv_val.
     simpl in Hvalid_smapv_val.
     destruct Hvalid_smapv_val as [_ [Hvalid_arg1 [Hvalid_arg2 _]]].
-    simpl.
-    assumption.
+    simpl. unfold valid_stack_op_instr. simpl.
+    intuition.
   * destruct (fcmp arg2 (Val WZero) n sb n sb instk_height evm_stack_opm) 
-      eqn: eq_fcmp_arg2; try (injection Hoptm_add_0_sbinding as eq_val' eq_flag;
+      eqn: eq_fcmp_arg2; try (injection Hoptm_eq_zero_sbinding as eq_val' eq_flag;
       rewrite <- eq_val'; assumption).
-    injection Hoptm_add_0_sbinding as eq_val' eq_flag.
+    injection Hoptm_eq_zero_sbinding as eq_val' eq_flag.
     rewrite <- eq_val'.
     simpl in Hvalid_smapv_val. unfold valid_stack_op_instr in Hvalid_smapv_val.
     simpl in Hvalid_smapv_val.
     destruct Hvalid_smapv_val as [_ [Hvalid_arg1 [Hvalid_arg2 _]]].
-    simpl.
-    assumption.
-  + injection Hoptm_add_0_sbinding as eq_val' eq_flag.
+    simpl. unfold valid_stack_op_instr. simpl.
+    intuition.
+  + injection Hoptm_eq_zero_sbinding as eq_val' eq_flag.
     rewrite <- eq_val'.
     assumption.
-  + injection Hoptm_add_0_sbinding as eq_val' eq_flag.
+  + injection Hoptm_eq_zero_sbinding as eq_val' eq_flag.
     rewrite <- eq_val'.
     assumption.
-  + injection Hoptm_add_0_sbinding as eq_val' eq_flag.
+  + injection Hoptm_eq_zero_sbinding as eq_val' eq_flag.
     rewrite <- eq_val'.
     assumption.
 Qed.
 
 
-Lemma evm_add_zero_l: forall ctx v,
-evm_add ctx [WZero; v] = v.
-Proof.
-intros ctx v. simpl.
-rewrite -> wplus_wzero_2.
-reflexivity.
-Qed.
-
-
-Lemma evm_add_zero_r: forall ctx v,
-evm_add ctx [v; WZero] = v.
-Proof.
-intros ctx v. simpl.
-rewrite -> wplus_wzero_1.
-reflexivity.
-Qed.
-
-
-Lemma optimize_add_0_sbinding_snd:
-opt_sbinding_snd optimize_add_0_sbinding.
+Lemma optimize_eq_zero_sbinding_snd:
+opt_sbinding_snd optimize_eq_zero_sbinding.
 Proof.
 unfold opt_sbinding_snd.
 intros val val' fcmp sb maxidx instk_height idx flag Hsafe_sstack_val_cmp
-  Hvalid Hoptm_add_0_sbinding.
+  Hvalid Hoptm_eq_zero_sbinding.
 split.
 - (* valid_sbindings *)
-  apply valid_bindings_snd_opt with (val:=val)(opt:=optimize_add_0_sbinding)
+  apply valid_bindings_snd_opt with (val:=val)(opt:=optimize_eq_zero_sbinding)
     (fcmp:=fcmp)(flag:=flag); try assumption.
-  apply optimize_add_0_sbinding_smapv_valid. 
+  apply optimize_eq_zero_sbinding_smapv_valid. 
     
 - (* evaluation is preserved *) 
   intros stk mem strg ctx v Hlen Heval_orig.
   assert (Hlen2 := Hlen).
   rewrite -> Hlen in Hlen2.
   rewrite <- Hlen in Hlen2 at 2.
-  unfold optimize_add_0_sbinding in Hoptm_add_0_sbinding.
+  unfold optimize_eq_zero_sbinding in Hoptm_eq_zero_sbinding.
   pose proof (Hvalid_maxidx instk_height maxidx idx val sb evm_stack_opm
       Hvalid) as eq_maxidx_idx.
   destruct val as [vv|vv|label args|offset smem|key sstrg|offset seze smem]
-    eqn: eq_val; try inject_rw Hoptm_add_0_sbinding eq_val'.
+    eqn: eq_val; try inject_rw Hoptm_eq_zero_sbinding eq_val'.
   (* SymOp label args *)
-  destruct label; try inject_rw Hoptm_add_0_sbinding eq_val'.
+  destruct label; try inject_rw Hoptm_eq_zero_sbinding eq_val'.
   destruct args as [|arg1 r1] eqn: eq_args; 
-    try inject_rw Hoptm_add_0_sbinding eq_val'.
+    try inject_rw Hoptm_eq_zero_sbinding eq_val'.
   destruct r1 as [|arg2 r2] eqn: eq_r1; 
-    try inject_rw Hoptm_add_0_sbinding eq_val'.
-  destruct r2 as [|arg3 r3] eqn: eq_r2; 
-    try inject_rw Hoptm_add_0_sbinding eq_val'.
+    try inject_rw Hoptm_eq_zero_sbinding eq_val'.
+  destruct r2; try inject_rw Hoptm_eq_zero_sbinding eq_val'.
   destruct (fcmp arg1 (Val WZero) idx sb idx sb instk_height) 
     eqn: fcmp_arg1_zero.
   + (* arg1 ~ WZero *)
-    injection Hoptm_add_0_sbinding as eq_val' _. 
+    injection Hoptm_eq_zero_sbinding as eq_val' _. 
     rewrite <- eq_val'.
     unfold eval_sstack_val in Heval_orig. simpl in Heval_orig.
     rewrite -> PeanoNat.Nat.eqb_refl in Heval_orig.
@@ -230,63 +225,64 @@ split.
     injection Heval_vzero as eq_vzero.
     rewrite <- eq_varg1 in Heval_orig.
     rewrite <- eq_vzero in Heval_orig.
-    rewrite -> evm_add_zero_l in Heval_orig.
+    simpl. rewrite -> PeanoNat.Nat.eqb_refl.
+    simpl. rewrite -> eval_arg2. 
     rewrite <- Heval_orig.
-    rewrite <- eval_sstack_val'_freshvar.
-    apply eval_sstack_val'_preserved_when_depth_extended in eval_arg2.
-    apply eval'_maxidx_indep with (n:=idx).
-    assumption.
+    
+    rewrite -> eq_zero_iszero1.
+    reflexivity.
+
   + (* arg2 ~ WZero *)
     destruct (fcmp arg2 (Val WZero) idx sb idx sb instk_height evm_stack_opm)
-      eqn: fcmp_arg2_zero.
-    * injection Hoptm_add_0_sbinding as eq_val' _.
-      rewrite <- eq_val'.
-      unfold eval_sstack_val in Heval_orig.
-      simpl in Heval_orig.
-      rewrite -> PeanoNat.Nat.eqb_refl in Heval_orig.
-      simpl in Heval_orig.
-      destruct (eval_sstack_val' maxidx arg1 stk mem strg ctx idx sb 
-        evm_stack_opm) as [varg1|] eqn: eval_arg1; try discriminate.
-      destruct (eval_sstack_val' maxidx arg2 stk mem strg ctx idx sb 
-        evm_stack_opm) as [varg2|] eqn: eval_arg2; try discriminate.
-      unfold safe_sstack_val_cmp in Hsafe_sstack_val_cmp.
+      eqn: fcmp_arg2_zero; try (injection Hoptm_eq_zero_sbinding as eq_val'; 
+                                rewrite <- eq_val';
+                                assumption).
+    injection Hoptm_eq_zero_sbinding as eq_val' _.
+    rewrite <- eq_val'.
+    unfold eval_sstack_val in Heval_orig.
+    simpl in Heval_orig.
+    rewrite -> PeanoNat.Nat.eqb_refl in Heval_orig.
+    simpl in Heval_orig.
+    destruct (eval_sstack_val' maxidx arg1 stk mem strg ctx idx sb 
+      evm_stack_opm) as [varg1|] eqn: eval_arg1; try discriminate.
+    destruct (eval_sstack_val' maxidx arg2 stk mem strg ctx idx sb 
+      evm_stack_opm) as [varg2|] eqn: eval_arg2; try discriminate.
+    unfold safe_sstack_val_cmp in Hsafe_sstack_val_cmp.
       
-      unfold valid_bindings in Hvalid.
-      destruct Hvalid as [eq_maxid [Hvalid_smap_value Hvalid_bindings_sb]].
-      unfold valid_smap_value in Hvalid_smap_value.
-      unfold valid_stack_op_instr in Hvalid_smap_value.
-      simpl in Hvalid_smap_value.
-      destruct (Hvalid_smap_value) as [_ [Hvalid_arg1 [Hvalid_arg2 _ ]]].
-      fold valid_bindings in Hvalid_bindings_sb.
+    unfold valid_bindings in Hvalid.
+    destruct Hvalid as [eq_maxid [Hvalid_smap_value Hvalid_bindings_sb]].
+    unfold valid_smap_value in Hvalid_smap_value.
+    unfold valid_stack_op_instr in Hvalid_smap_value.
+    simpl in Hvalid_smap_value.
+    destruct (Hvalid_smap_value) as [_ [Hvalid_arg1 [Hvalid_arg2 _ ]]].
+    fold valid_bindings in Hvalid_bindings_sb.
       
-      pose proof (valid_sstack_value_const instk_height idx v) as 
-        Hvalid_zero.
-      pose proof (Hsafe_sstack_val_cmp arg2 (Val WZero) idx sb idx sb 
-        instk_height evm_stack_opm Hvalid_arg2 Hvalid_zero Hvalid_bindings_sb
-        Hvalid_bindings_sb fcmp_arg2_zero stk mem strg ctx Hlen2)
-        as [vzero [Heval_arg2 Heval_vzero]].
-      assert (Heval_arg2_copy := Heval_arg2).
-      unfold eval_sstack_val in Heval_arg2_copy.
-      rewrite -> eval_sstack_val_const in Heval_vzero.
-      rewrite <- Heval_vzero in Heval_arg2.
+    pose proof (valid_sstack_value_const instk_height idx v) as 
+      Hvalid_zero.
+    pose proof (Hsafe_sstack_val_cmp arg2 (Val WZero) idx sb idx sb 
+      instk_height evm_stack_opm Hvalid_arg2 Hvalid_zero Hvalid_bindings_sb
+      Hvalid_bindings_sb fcmp_arg2_zero stk mem strg ctx Hlen2)
+      as [vzero [Heval_arg2 Heval_vzero]].
+    assert (Heval_arg2_copy := Heval_arg2).
+    unfold eval_sstack_val in Heval_arg2_copy.
+    rewrite -> eval_sstack_val_const in Heval_vzero.
+    rewrite <- Heval_vzero in Heval_arg2.
     
-      unfold eval_sstack_val.
-      rewrite -> eq_maxid in eval_arg2.
-      rewrite -> Heval_arg2_copy in eval_arg2.
-      injection eval_arg2 as eq_varg2.
-      injection Heval_vzero as eq_vzero.
-      rewrite <- eq_varg2 in Heval_orig.
-      rewrite <- eq_vzero in Heval_orig.
-      rewrite -> evm_add_zero_r in Heval_orig.
-      rewrite <- Heval_orig.
-      rewrite <- eval_sstack_val'_freshvar.
-      apply eval_sstack_val'_preserved_when_depth_extended in eval_arg1.
-      apply eval'_maxidx_indep with (n:=idx).
-      assumption.
-    * injection Hoptm_add_0_sbinding as eq_val' _. 
-      rewrite <- eq_val'.
-      assumption.
+    unfold eval_sstack_val.
+    rewrite -> eq_maxid in eval_arg2.
+    rewrite -> Heval_arg2_copy in eval_arg2.
+    injection eval_arg2 as eq_varg2.
+    injection Heval_vzero as eq_vzero.
+    rewrite <- eq_varg2 in Heval_orig.
+    rewrite <- eq_vzero in Heval_orig.
+    simpl.
+    simpl. rewrite -> PeanoNat.Nat.eqb_refl.
+    simpl. rewrite -> eval_arg1. 
+    rewrite <- Heval_orig.
+    
+    rewrite -> eq_zero_iszero2.
+    reflexivity.
 Qed.
 
 
-End Opt_add_zero.
+End Opt_eq_zero.
