ver2/optimizations/mul_shl.v
@@ -94,26 +94,6 @@ match val with
 end.
 
 
-Lemma pow2_shl: forall x,
-wlshift WOne x = natToWord EVMWordSize (2 ^ x).
-Proof.
-induction x as [|x' IH].
-- simpl. rewrite -> wlshift_0. reflexivity.
-- rewrite -> wlshift_mul_pow2. 
-  rewrite -> wmult_unit.
-  reflexivity.
-Qed.
-
-Search wlshift'.
-Lemma pow2_shl': forall x,
-wlshift' WOne x = natToWord EVMWordSize (2 ^ x).
-Proof.
-intros x.
-rewrite -> wlshift_alt.
-apply pow2_shl.
-Qed.
-
-
 Lemma wmult_shl_1: forall x y,
 wmult (wlshift WOne x) y = wlshift y x.
 Proof.
@@ -135,21 +115,11 @@ apply wmult_shl_1.
 Qed.
 
 
-Lemma lenght2: forall {T: Type} (x y: T), (length [x; y] =? 2) = true.
-Proof.
-intros T x y.
-reflexivity.
-Qed.
-
-Search follow_in_smap.
-Search valid_sstack_value.
-
-
 Lemma optimize_mul_shl_sbinding_smapv_valid:
 opt_smapv_valid_snd optimize_mul_shl_sbinding.
 Proof.
 unfold opt_smapv_valid_snd.
-intros instk_height n ops fcmp sb val val' flag.
+intros instk_height n fcmp sb val val' flag.
 intros Hvalid_smapv_val Hvalid Hoptm_sbinding.
 unfold optimize_mul_shl_sbinding in Hoptm_sbinding.
 destruct (val) as [basicv|pushtagv|label args|offset smem|key sstrg|
@@ -157,9 +127,9 @@ destruct (val) as [basicv|pushtagv|label args|offset smem|key sstrg|
   try inject_rw Hoptm_sbinding eq_val'.
 destruct label eqn: eq_label; try try inject_rw Hoptm_sbinding eq_val'.
 destruct args as [|arg1 r1]; try inject_rw Hoptm_sbinding eq_val'.
-destruct r1 as [|y r2]; try inject_rw Hoptm_sbinding eq_val'.
+destruct r1 as [|arg2 r2]; try inject_rw Hoptm_sbinding eq_val'.
 destruct r2; try inject_rw Hoptm_sbinding eq_val'.
-destruct (is_shl_1 arg1 fcmp n instk_height sb ops) as [x|] eqn: is_shl_arg1.
+destruct (is_shl_1 arg1 fcmp n instk_height sb evm_stack_opm) as [x|] eqn: is_shl_arg1.
 - injection Hoptm_sbinding as eq_val' _.
   rewrite <- eq_val'.
   unfold is_shl_1 in is_shl_arg1.
@@ -171,23 +141,23 @@ destruct (is_shl_1 arg1 fcmp n instk_height sb ops) as [x|] eqn: is_shl_arg1.
   destruct args2 as [|xx r2]; try discriminate.
   destruct r2 as [|onev r2']; try discriminate.
   destruct r2'; try discriminate.
-  destruct (fcmp onev (Val WOne) n sb n sb instk_height ops) eqn: fcmp_onev;
+  destruct (fcmp onev (Val WOne) n sb n sb instk_height evm_stack_opm) eqn: fcmp_onev;
     try discriminate.
     
   simpl in Hvalid_smapv_val. unfold valid_stack_op_instr in Hvalid_smapv_val.
-  destruct (ops MUL) as [nargs_mult fmult Hcomm_mult Hctx_indep_mult].
-  destruct Hvalid_smapv_val as [_ Hvalid_sstack_arg1_y].
-  unfold valid_sstack in Hvalid_sstack_arg1_y.
-  destruct Hvalid_sstack_arg1_y as [Hvalid_arg1 [Hvalid_y _]].
+  simpl in Hvalid_smapv_val.
+  destruct Hvalid_smapv_val as [_ Hvalid_sstack_arg1_arg2].
+  unfold valid_sstack in Hvalid_sstack_arg1_arg2.
+  destruct Hvalid_sstack_arg1_arg2 as [Hvalid_arg1 [Hvalid_arg2 _]].
   injection is_shl_arg1 as eq_xx. rewrite -> eq_xx in Hfollow_arg1.
-  pose proof (valid_follow_in_smap sb arg1 instk_height n ops
+  pose proof (valid_follow_in_smap sb arg1 instk_height n evm_stack_opm
     (SymOp SHL [x; onev]) idx' sb' Hvalid_arg1 Hvalid Hfollow_arg1) as Himpl.
   destruct Himpl as [Hvalid_shl [Hvalid_sb' Himpl]].
   pose proof (not_basic_value_smv_symop SHL [x;onev]) as Hnot_basic.
   apply Himpl in Hnot_basic.
   unfold valid_smap_value in Hvalid_shl. 
   unfold valid_stack_op_instr in Hvalid_shl.
-  destruct (ops SHL) as [nargs f Hcomm Hctx] eqn: eq_ops_shl.
+  simpl in Hvalid_shl.
   destruct Hvalid_shl as [Hnargs Hvalid_idx'].
   simpl in Hnargs.
   unfold valid_sstack in Hvalid_idx'.
@@ -195,31 +165,65 @@ destruct (is_shl_1 arg1 fcmp n instk_height sb ops) as [x|] eqn: is_shl_arg1.
   apply valid_sstack_value_gt with (m:=n) in Hvalid_x; try assumption.
   
   simpl. unfold valid_stack_op_instr.
-  rewrite -> eq_ops_shl.
-  rewrite <- Hnargs. simpl.
+  simpl. 
   intuition.
-- destruct (is_shl_1 y fcmp n instk_height sb ops) eqn: is_shl_arg2;
+- destruct (is_shl_1 arg2 fcmp n instk_height sb evm_stack_opm) as [y|] eqn: is_shl_arg2;
     try inject_rw Hoptm_sbinding eq_val'.
-  (*TODO*)
-Admitted.
+  injection Hoptm_sbinding as eq_val' _.
+  rewrite <- eq_val'.
+  unfold is_shl_1 in is_shl_arg2.
+  destruct (follow_in_smap arg2 n sb) as [fsmv2|] eqn: Hfollow_arg2;
+    try discriminate.
+  destruct fsmv2 as [smv_arg2 idx' sb'].
+  destruct (smv_arg2) as [_1|_2|label2 args2|_4|_5|_6]; try discriminate.
+  destruct label2; try discriminate.
+  destruct args2 as [|yy r2]; try discriminate.
+  destruct r2 as [|onev r2']; try discriminate.
+  destruct r2'; try discriminate.
+  destruct (fcmp onev (Val WOne) n sb n sb instk_height evm_stack_opm) eqn: fcmp_onev;
+    try discriminate.
+    
+  simpl in Hvalid_smapv_val. unfold valid_stack_op_instr in Hvalid_smapv_val.
+  simpl in Hvalid_smapv_val.
+  destruct Hvalid_smapv_val as [_ Hvalid_sstack_arg1_arg2].
+  unfold valid_sstack in Hvalid_sstack_arg1_arg2.
+  destruct Hvalid_sstack_arg1_arg2 as [Hvalid_arg1 [Hvalid_arg2 _]].
+  injection is_shl_arg2 as eq_yy. rewrite -> eq_yy in Hfollow_arg2.
+  pose proof (valid_follow_in_smap sb arg2 instk_height n evm_stack_opm
+    (SymOp SHL [y; onev]) idx' sb' Hvalid_arg2 Hvalid Hfollow_arg2) as Himpl.
+  destruct Himpl as [Hvalid_shl [Hvalid_sb' Himpl]].
+  pose proof (not_basic_value_smv_symop SHL [y;onev]) as Hnot_basic.
+  apply Himpl in Hnot_basic.
+  unfold valid_smap_value in Hvalid_shl. 
+  unfold valid_stack_op_instr in Hvalid_shl.
+  simpl in Hvalid_shl.
+  destruct Hvalid_shl as [Hnargs Hvalid_idx'].
+  simpl in Hnargs.
+  unfold valid_sstack in Hvalid_idx'.
+  destruct Hvalid_idx' as [Hvalid_y _].
+  apply valid_sstack_value_gt with (m:=n) in Hvalid_y; try assumption.
+  
+  simpl. unfold valid_stack_op_instr.
+  simpl. 
+  intuition.
+Qed.
 
 
 Lemma optimize_mul_shl_sbinding_snd:
 opt_sbinding_snd optimize_mul_shl_sbinding.
 Proof.
-(*
 unfold opt_sbinding_snd.
 intros val val' fcmp sb maxidx instk_height idx flag Hsafe_sstack_val_cmp
   Hvalid Hoptm_sbinding.
 split.
 - (* valid_sbindings *)
-  apply valid_bindings_snd_opt with (val:=val)(opt:=optimize_and_origin_sbinding)
+  apply valid_bindings_snd_opt with (val:=val)(opt:=optimize_mul_shl_sbinding)
     (fcmp:=fcmp)(flag:=flag); try assumption.
-  apply optimize_and_origin_sbinding_smapv_valid. 
+  apply optimize_mul_shl_sbinding_smapv_valid. 
 
 - (* evaluation is preserved *) 
   intros stk mem strg ctx v Hlen Heval_orig.
-  unfold optimize_and_origin_sbinding in Hoptm_sbinding.
+  unfold optimize_mul_shl_sbinding in Hoptm_sbinding.
   destruct val as [vv|vv|label args|offset smem|key sstrg|offset seze smem]
     eqn: eq_val; try inject_rw Hoptm_sbinding eq_val'.
   (* SymOp label args *)
@@ -228,133 +232,175 @@ split.
     try inject_rw Hoptm_sbinding eq_val'.
   destruct r1 as [|arg2 r2]; try inject_rw Hoptm_sbinding eq_val'.
   destruct r2; try inject_rw Hoptm_sbinding eq_val'.
-  destruct (is_origin_mask arg1 arg2 fcmp idx instk_height sb evm_stack_opm
-         || is_origin_mask arg2 arg1 fcmp idx instk_height sb evm_stack_opm)
-    eqn: eq_is_origin; try inject_rw Hoptm_sbinding eq_val'.
-  unfold orb in eq_is_origin.
-  destruct (is_origin_mask arg1 arg2 fcmp idx instk_height sb evm_stack_opm)
-    eqn: is_origin_arg1_arg2.
-  + unfold is_origin_mask in is_origin_arg1_arg2.
-    destruct (follow_in_smap arg1 idx sb) as [fsmv|] eqn: eq_follow_arg1;
-      try discriminate.
-    destruct fsmv as [smv idx' sb'] eqn: eq_fsmv.
-    destruct smv as [_1|_2|label2 args2|_4|_5|_6] eqn: eq_smv;
-      try discriminate.
-    destruct label2 eqn: eq_label2; try discriminate.
-    destruct args2 as [|arg11 r21]; try discriminate.
-    
-    injection Hoptm_sbinding as eq_val' _.
+  destruct (is_shl_1 arg1 fcmp idx instk_height sb evm_stack_opm) 
+    as [x|] eqn: is_shl_arg1.
+  + injection Hoptm_sbinding as eq_val' _.
     rewrite <- eq_val'.
-    
-    unfold eval_sstack_val in Heval_orig.
-    simpl in Heval_orig.
+    unfold is_shl_1 in is_shl_arg1.
+    destruct (follow_in_smap arg1 idx sb) as [fsmv1|] eqn: Hfollow_arg1;
+      try discriminate.
+    destruct fsmv1 as [smv_arg1 idx' sb'].
+    destruct (smv_arg1) as [_1|_2|label2 args2|_4|_5|_6]; try discriminate.
+    destruct label2; try discriminate.
+    destruct args2 as [|xx r2]; try discriminate.
+    destruct r2 as [|onev r2']; try discriminate.
+    destruct r2'; try discriminate.
+    destruct (fcmp onev (Val WOne) idx sb idx sb instk_height evm_stack_opm) eqn: fcmp_onev;
+      try discriminate.
+      
+    unfold eval_sstack_val in Heval_orig. simpl in Heval_orig.
     rewrite -> PeanoNat.Nat.eqb_refl in Heval_orig.
     simpl in Heval_orig.
     destruct (eval_sstack_val' maxidx arg1 stk mem strg ctx idx sb 
-      evm_stack_opm) as [arg1v|] eqn: eq_eval_arg1; try discriminate.
+      evm_stack_opm) as [arg1v|] eqn: eval_arg1; try discriminate.
     destruct (eval_sstack_val' maxidx arg2 stk mem strg ctx idx sb
-      evm_stack_opm) as [arg2v|] eqn: eq_eval_arg2; try discriminate.
-    injection Heval_orig as eq_v. rewrite <- eq_v.
+      evm_stack_opm) as [arg2v|] eqn: eval_arg2; try discriminate.
+    rewrite <- Heval_orig. simpl.
     
     unfold eval_sstack_val. simpl.
     rewrite -> PeanoNat.Nat.eqb_refl. simpl.
-    unfold evm_origin.
-    unfold eval_sstack_val' in eq_eval_arg1.
+    rewrite -> eval_arg2.
     destruct maxidx as [|maxidx'] eqn: eq_maxidx; try discriminate.
-    rewrite -> eq_follow_arg1 in eq_eval_arg1. simpl in eq_eval_arg1.
-    injection eq_eval_arg1 as eq_arg1v. 
-    rewrite <- eq_arg1v. unfold evm_origin.
+    unfold eval_sstack_val' in eval_arg1.
+    rewrite -> Hfollow_arg1 in eval_arg1.
+    simpl in eval_arg1. fold eval_sstack_val' in eval_arg1.
+    destruct (eval_sstack_val' maxidx' xx stk mem strg ctx idx' sb'
+      evm_stack_opm) as [xxv|] eqn: eval_xx_sb'; try discriminate.
+    destruct (eval_sstack_val' maxidx' onev stk mem strg ctx idx' sb'
+      evm_stack_opm) as [onev_v|] eqn: eval_onev; try discriminate.
+    injection is_shl_arg1 as eq_xx. rewrite -> eq_xx in eval_xx_sb'.
+    injection eval_arg1 as eq_arg1v. rewrite <- eq_arg1v.
     
-    unfold safe_sstack_val_cmp in Hsafe_sstack_val_cmp.
-    pose proof (valid_sstack_value_const instk_height idx two_exp_160_minus_1)
-      as valid_sstack_two_exp_160_minus_1.
     simpl in Hvalid.
-    destruct Hvalid as [eq_idx [Hvalid_stack_op Hvalid_sb]].
-    unfold valid_stack_op_instr in Hvalid_stack_op.
-    simpl in Hvalid_stack_op.
-    destruct Hvalid_stack_op as [_ [Hvalid_arg1 [Hvalid_arg2 _]]].
+    destruct Hvalid as [eq_maxidx' [Hvalid_arg1_arg2 Hvalid_sb]].
+    unfold valid_stack_op_instr in Hvalid_arg1_arg2.
+    simpl in Hvalid_arg1_arg2.
+    destruct Hvalid_arg1_arg2 as [_ [Hvalid_arg1 [Hvalid_arg2 _]]].
+    pose proof (follow_suffix sb arg1 idx (SymOp SHL [xx; onev]) idx' sb'
+      Hfollow_arg1) as [prefix sb_prefix].
+    rewrite -> eval'_maxidx_indep_eq with (m:=idx) in eval_xx_sb'.
+    pose proof (eval_sstack_val'_extend_sb instk_height maxidx' stk mem strg
+      ctx idx sb sb' evm_stack_opm prefix Hvalid_sb sb_prefix x xxv
+      eval_xx_sb') as eval_x_sb.
+    apply eval_sstack_val'_preserved_when_depth_extended in eval_x_sb.
+    rewrite -> eval_x_sb. 
     
+    pose proof (valid_follow_in_smap sb arg1 instk_height idx evm_stack_opm
+      (SymOp SHL [xx; onev]) idx' sb' Hvalid_arg1 Hvalid_sb Hfollow_arg1)
+      as [Hvalid_smv [Hvalid_sb' Himpl]].
+    pose proof (not_basic_value_smv_symop SHL [xx;onev]) as Hnot_basic.
+    apply Himpl in Hnot_basic as idx_gt_idx'.
+    unfold valid_smap_value in Hvalid_smv.
+    unfold valid_stack_op_instr in Hvalid_smv.
+    simpl in Hvalid_smv.
+    destruct Hvalid_smv as [_ [Hvalid_xx [Hvalid_onev _]]].
+    pose proof (valid_sstack_value_gt instk_height idx' idx onev Hvalid_onev
+      idx_gt_idx') as Hvalid_onev_sb.
     symmetry in Hlen.
-    pose proof (Hsafe_sstack_val_cmp arg2 (Val two_exp_160_minus_1) idx sb
-      idx sb instk_height evm_stack_opm Hvalid_arg2 
-      valid_sstack_two_exp_160_minus_1 Hvalid_sb Hvalid_sb is_origin_arg1_arg2
-      stk mem strg ctx Hlen) as eval_arg2_two_exp.
-    destruct eval_arg2_two_exp as [vv [eval_arg2_vv eval_two_exp_vv]].
-    unfold eval_sstack_val in eval_arg2_vv.
-    unfold eval_sstack_val in eval_two_exp_vv.
-    rewrite -> eq_idx in eq_eval_arg2.
-    rewrite -> eval_sstack_val'_const in eval_two_exp_vv.
-    rewrite -> eq_eval_arg2 in eval_arg2_vv.
-    rewrite <- eval_arg2_vv in eval_two_exp_vv.
-    injection eval_two_exp_vv as eq_vv.
-    rewrite <- eq_vv.
+    pose proof (valid_sstack_value_const instk_height idx WOne) as Hvalid_WOne.
+    pose proof (Hsafe_sstack_val_cmp onev (Val WOne) idx sb idx sb instk_height
+      evm_stack_opm Hvalid_onev_sb Hvalid_WOne Hvalid_sb Hvalid_sb fcmp_onev
+      stk mem strg ctx Hlen) as [vv [eval_onev' eval_WOne]].
+    rewrite -> eval_sstack_val_const in eval_WOne.
+    rewrite <- eval_WOne in eval_onev'.
+    unfold eval_sstack_val in eval_onev'.
+    apply eval_sstack_val'_preserved_when_depth_extended in eval_onev.
+    rewrite -> eq_maxidx' in eval_onev.
+    rewrite -> eval'_maxidx_indep_eq with (m:=idx) in eval_onev.
+    apply eval_sstack_val'_extend_sb with (instk_height:=instk_height)(sb:=sb)
+      (prefix:=prefix) in eval_onev; try assumption.
+    rewrite -> eval_onev' in eval_onev.
+    injection eval_onev as eq_onev_v.
+    rewrite <- eq_onev_v.
     
-    unfold two_exp_160_minus_1.
-    rewrite <- masking_address_extension_word.
-    reflexivity. 
-
-  + unfold is_origin_mask in eq_is_origin.
-    destruct (follow_in_smap arg2 idx sb) as [fsmv|] eqn: eq_follow_arg2;
-      try discriminate.
-    destruct fsmv as [smv idx' sb'] eqn: eq_fsmv.
-    destruct smv as [_1|_2|label2 args2|_4|_5|_6] eqn: eq_smv;
-      try discriminate.
-    destruct label2 eqn: eq_label2; try discriminate.
-    destruct args2 as [|arg11 r21]; try discriminate.
-    
+    simpl. rewrite <- wmult_shl'_1.
+    reflexivity.
+  + destruct (is_shl_1 arg2 fcmp idx instk_height sb evm_stack_opm) as [y|] 
+    eqn: is_shl_arg2; try inject_rw Hoptm_sbinding eq_val'.
     injection Hoptm_sbinding as eq_val' _.
     rewrite <- eq_val'.
-    
-    unfold eval_sstack_val in Heval_orig.
-    simpl in Heval_orig.
+    unfold is_shl_1 in is_shl_arg2.
+    destruct (follow_in_smap arg2 idx sb) as [fsmv2|] eqn: Hfollow_arg2;
+      try discriminate.
+    destruct fsmv2 as [smv_arg2 idx' sb'].
+    destruct (smv_arg2) as [_1|_2|label2 args2|_4|_5|_6]; try discriminate.
+    destruct label2; try discriminate.
+    destruct args2 as [|yy r2]; try discriminate.
+    destruct r2 as [|onev r2']; try discriminate.
+    destruct r2'; try discriminate.
+    destruct (fcmp onev (Val WOne) idx sb idx sb instk_height evm_stack_opm) 
+      eqn: fcmp_onev; try discriminate.
+      
+    unfold eval_sstack_val in Heval_orig. simpl in Heval_orig.
     rewrite -> PeanoNat.Nat.eqb_refl in Heval_orig.
     simpl in Heval_orig.
     destruct (eval_sstack_val' maxidx arg1 stk mem strg ctx idx sb 
-      evm_stack_opm) as [arg1v|] eqn: eq_eval_arg1; try discriminate.
+      evm_stack_opm) as [arg1v|] eqn: eval_arg1; try discriminate.
     destruct (eval_sstack_val' maxidx arg2 stk mem strg ctx idx sb
-      evm_stack_opm) as [arg2v|] eqn: eq_eval_arg2; try discriminate.
-    injection Heval_orig as eq_v. rewrite <- eq_v.
+      evm_stack_opm) as [arg2v|] eqn: eval_arg2; try discriminate.
+    rewrite <- Heval_orig. simpl.
     
     unfold eval_sstack_val. simpl.
     rewrite -> PeanoNat.Nat.eqb_refl. simpl.
-    unfold evm_origin.
-    unfold eval_sstack_val' in eq_eval_arg2.
+    rewrite -> eval_arg1.
     destruct maxidx as [|maxidx'] eqn: eq_maxidx; try discriminate.
-    rewrite -> eq_follow_arg2 in eq_eval_arg2. simpl in eq_eval_arg2.
-    injection eq_eval_arg2 as eq_arg2v. 
-    rewrite <- eq_arg2v. unfold evm_origin.
+    unfold eval_sstack_val' in eval_arg2.
+    rewrite -> Hfollow_arg2 in eval_arg2.
+    simpl in eval_arg2. fold eval_sstack_val' in eval_arg2.
+    destruct (eval_sstack_val' maxidx' yy stk mem strg ctx idx' sb'
+      evm_stack_opm) as [yyv|] eqn: eval_yy_sb'; try discriminate.
+    destruct (eval_sstack_val' maxidx' onev stk mem strg ctx idx' sb'
+      evm_stack_opm) as [onev_v|] eqn: eval_onev; try discriminate.
+    injection is_shl_arg2 as eq_yy. rewrite -> eq_yy in eval_yy_sb'.
+    injection eval_arg2 as eq_arg2v. rewrite <- eq_arg2v.
     
-    unfold safe_sstack_val_cmp in Hsafe_sstack_val_cmp.
-    pose proof (valid_sstack_value_const instk_height idx two_exp_160_minus_1)
-      as valid_sstack_two_exp_160_minus_1.
     simpl in Hvalid.
-    destruct Hvalid as [eq_idx [Hvalid_stack_op Hvalid_sb]].
-    unfold valid_stack_op_instr in Hvalid_stack_op.
-    simpl in Hvalid_stack_op.
-    destruct Hvalid_stack_op as [_ [Hvalid_arg1 [Hvalid_arg2 _]]].
+    destruct Hvalid as [eq_maxidx' [Hvalid_arg1_arg2 Hvalid_sb]].
+    unfold valid_stack_op_instr in Hvalid_arg1_arg2.
+    simpl in Hvalid_arg1_arg2.
+    destruct Hvalid_arg1_arg2 as [_ [Hvalid_arg1 [Hvalid_arg2 _]]].
+    pose proof (follow_suffix sb arg2 idx (SymOp SHL [yy; onev]) idx' sb'
+      Hfollow_arg2) as [prefix sb_prefix].
+    rewrite -> eval'_maxidx_indep_eq with (m:=idx) in eval_yy_sb'.
+    pose proof (eval_sstack_val'_extend_sb instk_height maxidx' stk mem strg
+      ctx idx sb sb' evm_stack_opm prefix Hvalid_sb sb_prefix y yyv
+      eval_yy_sb') as eval_y_sb.
+    apply eval_sstack_val'_preserved_when_depth_extended in eval_y_sb.
+    rewrite -> eval_y_sb.
+    simpl. 
     
+    pose proof (valid_follow_in_smap sb arg2 instk_height idx evm_stack_opm
+      (SymOp SHL [yy; onev]) idx' sb' Hvalid_arg2 Hvalid_sb Hfollow_arg2)
+      as [Hvalid_smv [Hvalid_sb' Himpl]].
+    pose proof (not_basic_value_smv_symop SHL [yy;onev]) as Hnot_basic.
+    apply Himpl in Hnot_basic as idx_gt_idx'.
+    unfold valid_smap_value in Hvalid_smv.
+    unfold valid_stack_op_instr in Hvalid_smv.
+    simpl in Hvalid_smv.
+    destruct Hvalid_smv as [_ [Hvalid_yy [Hvalid_onev _]]].
+    pose proof (valid_sstack_value_gt instk_height idx' idx onev Hvalid_onev
+      idx_gt_idx') as Hvalid_onev_sb.
     symmetry in Hlen.
-    pose proof (Hsafe_sstack_val_cmp arg1 (Val two_exp_160_minus_1) idx sb
-      idx sb instk_height evm_stack_opm Hvalid_arg1 
-      valid_sstack_two_exp_160_minus_1 Hvalid_sb Hvalid_sb eq_is_origin
-      stk mem strg ctx Hlen) as eval_arg1_two_exp.
-    destruct eval_arg1_two_exp as [vv [eval_arg1_vv eval_two_exp_vv]].
-    unfold eval_sstack_val in eval_arg1_vv.
-    unfold eval_sstack_val in eval_two_exp_vv.
-    rewrite -> eq_idx in eq_eval_arg1.
-    rewrite -> eval_sstack_val'_const in eval_two_exp_vv.
-    rewrite -> eq_eval_arg1 in eval_arg1_vv.
-    rewrite <- eval_arg1_vv in eval_two_exp_vv.
-    injection eval_two_exp_vv as eq_vv.
-    rewrite <- eq_vv.
+    pose proof (valid_sstack_value_const instk_height idx WOne) as Hvalid_WOne.
+    pose proof (Hsafe_sstack_val_cmp onev (Val WOne) idx sb idx sb instk_height
+      evm_stack_opm Hvalid_onev_sb Hvalid_WOne Hvalid_sb Hvalid_sb fcmp_onev
+      stk mem strg ctx Hlen) as [vv [eval_onev' eval_WOne]].
+    rewrite -> eval_sstack_val_const in eval_WOne.
+    rewrite <- eval_WOne in eval_onev'.
+    unfold eval_sstack_val in eval_onev'.
+    apply eval_sstack_val'_preserved_when_depth_extended in eval_onev.
+    rewrite -> eq_maxidx' in eval_onev.
+    rewrite -> eval'_maxidx_indep_eq with (m:=idx) in eval_onev.
+    apply eval_sstack_val'_extend_sb with (instk_height:=instk_height)(sb:=sb)
+      (prefix:=prefix) in eval_onev; try assumption.
+    rewrite -> eval_onev' in eval_onev.
+    injection eval_onev as eq_onev_v.
+    rewrite <- eq_onev_v.
     
-    unfold two_exp_160_minus_1.
-    rewrite -> wand_comm.
-    rewrite <- masking_address_extension_word.
+    rewrite <- wmult_shl'_1.
+    rewrite -> wmult_comm.
     reflexivity.
 Qed.
-*)
-Admitted.
 
 
 End Opt_mul_shl.
