ver2/optimizations/shr_x_zero.v
@@ -1,0 +1,185 @@
+Require Import bbv.Word.
+Require Import Nat. 
+Require Import Coq.NArith.NArith.
+Require Import Coq.Bool.Bool.
+
+Require Import Coq.Logic.FunctionalExtensionality.
+
+Require Import FORVES.constants.
+Import Constants.
+
+Require Import FORVES.symbolic_state.
+Import SymbolicState.
+
+Require Import FORVES.symbolic_state_eval.
+Import SymbolicStateEval.
+
+Require Import FORVES.symbolic_state_cmp.
+Import SymbolicStateCmp.
+
+Require Import FORVES.valid_symbolic_state.
+Import ValidSymbolicState.
+
+Require Import FORVES.execution_state.
+Import ExecutionState.
+
+Require Import FORVES.stack_operation_instructions.
+Import StackOpInstrs.
+
+Require Import FORVES.program.
+Import Program.
+
+Require Import FORVES.symbolic_state_cmp_impl.
+Import SymbolicStateCmpImpl.
+
+Require Import FORVES.symbolic_state_eval_facts.
+Import SymbolicStateEvalFacts.
+
+Require Import FORVES.valid_symbolic_state.
+Import ValidSymbolicState.
+
+Require Import FORVES.misc.
+Import Misc.
+
+Require Import FORVES.eval_common.
+Import EvalCommon.
+
+Require Import FORVES.concrete_interpreter.
+Import ConcreteInterpreter.
+
+Require Import FORVES.optimizations_def.
+Import Optimizations_Def.
+
+Require Import FORVES.optimizations_common.
+Import Optimizations_Common.
+
+Require Import List.
+Import ListNotations.
+
+
+Module Opt_shr_x_zero.
+
+
+(* SHR(X, 0) = 0 *)
+Definition optimize_shr_x_zero_sbinding : opt_smap_value_type := 
+fun (val: smap_value) =>
+fun (fcmp: sstack_val_cmp_t) =>
+fun (sb: sbindings) =>
+fun (maxid: nat) =>
+fun (instk_height: nat) =>
+fun (ops: stack_op_instr_map) => 
+match val with
+| SymOp SHR [x; zero] => 
+  if fcmp zero (Val WZero) maxid sb maxid sb instk_height ops then 
+    (SymBasicVal (Val WZero), true)
+  else
+    (val, false)
+| _ => (val, false)
+end.
+
+
+(* For optimization SHR(X,0) = 0 *)
+Lemma shr_x_zero_equiv': forall (x: EVMWord),
+wdiv WZero (wlshift' WOne (wordToNat x)) = WZero.
+Proof.
+intros x.
+rewrite -> pow2_shl'.
+unfold wdiv. unfold wordBin.
+intuition.
+Qed.
+
+
+Lemma optimize_shr_x_zero_sbinding_smapv_valid:
+opt_smapv_valid_snd optimize_shr_x_zero_sbinding.
+Proof.
+unfold opt_smapv_valid_snd.
+intros instk_height n fcmp sb val val' flag.
+intros Hvalid_smapv_val Hvalid Hoptm_sbinding.
+unfold optimize_shr_x_zero_sbinding in Hoptm_sbinding.
+destruct (val) as [basicv|pushtagv|label args|offset smem|key sstrg|
+  offset size smem] eqn: eq_val; 
+  try inject_rw Hoptm_sbinding eq_val'.
+destruct label eqn: eq_label; try try inject_rw Hoptm_sbinding eq_val'.
+destruct args as [|x r1]; try inject_rw Hoptm_sbinding eq_val'.
+destruct r1 as [|zero r2]; try inject_rw Hoptm_sbinding eq_val'.
+destruct r2; try inject_rw Hoptm_sbinding eq_val'.
+destruct (fcmp zero (Val WZero) n sb n sb instk_height evm_stack_opm) 
+  eqn: fcmp_zero_WZero; try inject_rw Hoptm_sbinding eq_val'.
+injection Hoptm_sbinding as eq_val' _.
+rewrite <- eq_val'.
+simpl. 
+intuition.
+Qed.
+
+
+Lemma optimize_shr_x_zero_sbinding_snd:
+opt_sbinding_snd optimize_shr_x_zero_sbinding.
+Proof.
+unfold opt_sbinding_snd.
+intros val val' fcmp sb maxidx instk_height idx flag Hsafe_sstack_val_cmp
+  Hvalid Hoptm_sbinding.
+split.
+- (* valid_sbindings *)
+  apply valid_bindings_snd_opt with (val:=val)(opt:=optimize_shr_x_zero_sbinding)
+    (fcmp:=fcmp)(flag:=flag); try assumption.
+  apply optimize_shr_x_zero_sbinding_smapv_valid. 
+
+- (* evaluation is preserved *) 
+  intros stk mem strg ctx v Hlen Heval_orig.
+  unfold optimize_shr_x_zero_sbinding in Hoptm_sbinding.
+  destruct val as [vv|vv|label args|offset smem|key sstrg|offset seze smem]
+    eqn: eq_val; try inject_rw Hoptm_sbinding eq_val'.
+  (* SymOp label args *)
+  destruct label eqn: eq_label; try inject_rw Hoptm_sbinding eq_val'.
+  destruct args as [|x r1] eqn: eq_args; 
+    try inject_rw Hoptm_sbinding eq_val'.
+  destruct r1 as [|zero r2]; try inject_rw Hoptm_sbinding eq_val'.
+  destruct r2; try inject_rw Hoptm_sbinding eq_val'.
+  destruct (fcmp zero (Val WZero) idx sb idx sb instk_height evm_stack_opm)
+    eqn: fcmp_zero_WZero; try inject_rw Hoptm_sbinding eq_val'.
+  injection Hoptm_sbinding as eq_val' _.
+  rewrite <- eq_val'.
+      
+  unfold eval_sstack_val in Heval_orig. simpl in Heval_orig.
+  rewrite -> PeanoNat.Nat.eqb_refl in Heval_orig.
+  simpl in Heval_orig.
+  destruct (eval_sstack_val' maxidx x stk mem strg ctx idx sb 
+    evm_stack_opm) as [arg1v|] eqn: eval_arg1; try discriminate.
+  destruct (eval_sstack_val' maxidx zero stk mem strg ctx idx sb
+    evm_stack_opm) as [arg2v|] eqn: eval_arg2; try discriminate.
+  rewrite <- Heval_orig. simpl.
+  unfold eval_sstack_val.
+  rewrite <- eval_sstack_val'_freshvar.
+  rewrite -> eval_sstack_val'_const.
+  (*apply eval_sstack_val'_preserved_when_depth_extended in eval_arg2.
+  rewrite -> eval'_maxidx_indep_eq with (m:=maxidx) in eval_arg2.
+  rewrite -> eval_arg2.*)
+  
+  simpl in Hvalid. 
+  destruct Hvalid as [eq_maxid [Hvalid_smap_value Hvalid_bindings_sb]].
+  unfold valid_smap_value in Hvalid_smap_value.
+  unfold valid_stack_op_instr in Hvalid_smap_value.
+  simpl in Hvalid_smap_value.
+  destruct Hvalid_smap_value as [_ [Hvalid_arg1 [Hvalid_arg2 _ ]]].
+  pose proof (valid_sstack_value_const instk_height idx WZero) as valid_WZero.
+  symmetry in Hlen.
+  pose proof (Hsafe_sstack_val_cmp zero (Val WZero) idx sb idx sb instk_height
+    evm_stack_opm Hvalid_arg2 valid_WZero Hvalid_bindings_sb 
+    Hvalid_bindings_sb fcmp_zero_WZero stk mem strg ctx Hlen)
+    as [vv [eval_zero eval_wzero]].
+  unfold eval_sstack_val in eval_zero.
+  unfold eval_sstack_val in eval_wzero.
+  
+  rewrite -> eval_sstack_val'_const in eval_wzero.
+  rewrite <- eval_wzero in eval_zero.
+  rewrite <- eq_maxid in eval_zero.
+  rewrite -> eval_zero in eval_arg2.
+  injection eval_arg2 as eq_arg2v.
+  
+  rewrite <- eq_arg2v.
+  rewrite -> shr_x_zero_equiv'.
+  reflexivity.
+Qed.
+
+
+End Opt_shr_x_zero.
